Facts about de-duplication of lists.

Lib/ListSet.v
@@ -142,7 +142,7 @@ Proof.
 Qed.
 
 Corollary mem_list_cons {A:Type} (E:A->A->DProp) (x y:A) (l:list A) :
-  mem_list E x (y::l) <-> E x y \/ mem_list E x l.
+  eq_dprop (mem_list E x (y::l)) (E x y || mem_list E x l).
 Proof.
   split; cycle 1.
   { intros [h|h].
@@ -155,12 +155,12 @@ Proof.
 Qed.
 
 Lemma mem_list_app {A:Type} (E:A->A->DProp) (x:A) (l₁ l₂:list A) :
-  mem_list E x (l₁++l₂) <-> mem_list E x l₁ \/ mem_list E x l₂.
+  eq_dprop (mem_list E x (l₁++l₂)) (mem_list E x l₁ || mem_list E x l₂).
 Proof.
   induction l₁ as [|y l₁ hl₁].
-  + cbn [app]. intuition.
+  + cbn [app]. cbn -[mem_list]. intuition.
   + cbn [app]. rewrite !mem_list_cons,hl₁.
-    intuition.
+    cbn -[mem_list]. intuition.
 Qed.
 
 Program Fixpoint mem_of_mem_list {A:Type} (E:A->A->DProp) (l:list A) (x:A) : mem_list E x l -> Mem l :=
@@ -261,4 +261,103 @@ Instance mem_eq_set_list_proper A (E:A->A->DProp) (_:Transitive E) :
 Proof.
   intros x ? <- l₁ l₂ hl. unfold eq_dprop.
   eauto using mem_eq_set_list.
+Qed.
+
+
+(** * List without duplicates *)
+
+Fixpoint nodup {A} (R:A->A->DProp) (l:list A) : DProp :=
+  match l with
+  | [] => DTrue
+  | a::l => nodup R l && DNot (mem_list R a l)
+  end
+.
+
+Fixpoint deduplicate {A} (R:A->A->DProp) (l:list A) : list A :=
+  match l with
+  | [] => []
+  | a::l =>
+    let dl :=
+      List.filter
+        (fun x => if dec (DNot (R a x)) then true else false)
+        (deduplicate R l)
+    in
+    a::dl
+  end
+.
+
+Lemma filter_sub A R l (p:A->bool) :
+  forall x, mem_list R x (filter p l) -> mem_list R x l.
+Proof.
+  induction l as [|a l hl].
+  + cbn -[mem_list]. eauto.
+  + cbn -[mem_list]. intros x. destruct (p a).
+    * rewrite !mem_list_cons. cbn -[mem_list]. intuition.
+    * eauto using mem_list_right.
+Qed.
+
+Lemma filter_nodup A R (l:list A) : forall p:A->bool,
+  nodup R l -> nodup R (filter p l).
+Proof.
+  intros p.
+  induction l as [|a l hl].
+  + cbn. trivial.
+  + cbn -[mem_list]. destruct (p a).
+    * cbn -[mem_list]. rewrite !denies_spec.
+      intuition eauto using filter_sub.
+    * intuition.
+Qed.
+
+Lemma deduplicate_nodup A R (l:list A) : nodup R (deduplicate R l).
+Proof.
+  induction l as [ | a l hl].
+  + cbn. trivial.
+  + cbn -[DNot]. split.
+    * eauto using filter_nodup.
+    * revert hl. induction (deduplicate R l) as [|x l' hl'].
+      - cbn. auto.
+      - cbn -[DNot mem_list]. destruct dec as [hr|_];cycle 1.
+        { intuition. }
+        cbn -[mem_list] in *. rewrite mem_list_cons. cbn -[mem_list].
+        intuition.
+Qed.
+
+Lemma deduplicate_eq_set_list A (R:A->A->DProp) (l:list A) :
+  Equivalence R -> eq_set_list R l (deduplicate R l).
+Proof.
+  (* spiwack: This proof is much longer than it should be, reflecting
+     my dedication to avoiding equality… *)
+  intros e. cbn -[mem_list]. split.
+  + revert l. fix 2. intros l m.
+    refine match m with head a => _ | @tail _ _ l' m' => _ end.
+    * cbn [deduplicate of_mem].
+      apply mem_list_left. reflexivity.
+    * set (hl := deduplicate_eq_set_list _ m'). clearbody hl.
+      cbn [of_mem deduplicate].
+      rewrite mem_list_cons. cbn -[mem_list DNot].
+      generalize (deduplicate R l') (of_mem m') hl. clear -e.
+      { intros l. induction l as [|b l hl].
+        + eauto.
+        + intros x. cbn [filter].
+          destruct dec as [hr|hr].
+          * rewrite !mem_list_cons. cbn -[mem_list DNot].
+            intros [h|h].
+            - intuition.
+            - apply hl in h. intuition.
+          * rewrite mem_list_cons. cbn -[mem_list DNot]. cbn in hr.
+            intros [h|h].
+            - left. etransitivity. all:((idtac+symmetry);eassumption).
+            - intuition. }
+  + assert
+      (forall l x, mem_list R x (deduplicate R l) -> mem_list R x l) as incl.
+    { clear. intros l. induction l as [|a l hl].
+      + cbn -[mem_list]. eauto.
+      + intros x. cbn [deduplicate].
+        rewrite !mem_list_cons. cbn -[mem_list DNot].
+        intuition eauto using filter_sub. }
+    intros m. generalize l (deduplicate R l) m (incl l). clear -e.
+    intros l₁ l₂ m. induction m as [a l₂|a l₂ m hm].
+    * cbn -[mem_list]. intros h. apply h.
+      apply mem_list_left. reflexivity.
+    * cbn -[mem_list]. eauto using mem_list_right.
 Qed.
